<worksheet label="ws-act-1-3-5">
   <title>The Derivative of a Function at a Point - Activity 1.3.5</title>
    <activity xml:id="act-1-3-5" workspace="3cm">
 <introduction>
   <p>
    On a grid in <xref ref="emptygridact135"/>, sketch the graph of <m>f(x)=x^{2}-4</m> over <m>[-3,3]</m>.
    On another grid in <xref ref="emptygridact135"/>, sketch the graph of <m>g(x) = |x^{2}-4|</m> over <m>[-3,3]</m>.
  </p>
  
  <figure xml:id="emptygridact135" >
      <caption>Empty grids for plotting graphs of <m>f(x)=x^{2}-4</m> and <m>g(x) = |x^{2}-4|</m>.</caption>
      <sidebyside widths="40% 40%">
      <image>
        <latex-image>
\begin{tikzpicture}[thick,scale=1] 
\draw[step=1cm,color=gray!50] (-3,-4) grid (3,4);
   \draw [black!80,line width=0.5pt,-latex] (0,0) -- (3,0) node [below] at (2.75,0) {$x$};
   \draw [black!80,line width=0.5pt,-latex] (0,0) -- (-3,0);
   \draw [black!80,line width=0.5pt,-latex] (0,0) -- (0,4) node [right] at (0,3.75) {$y$};
   \draw [black!80,line width=0.5pt,-latex] (0,0) -- (0,-4);
\foreach \x/\xtext in { -2/-2, -1/-1, 1/1, 2/2}
    \draw[shift={(\x,0)}] (0pt,3pt) -- (0pt,-3pt); 
\foreach \y/\ytext in {-3/-3, -2/-2, -1/-1, 1/1, 2/2, 3/3}
    \draw[shift={(0,\y)}] (-2pt,0pt) -- (2pt,0pt); 
\end{tikzpicture}
    </latex-image>
  </image>
  <image>
      <latex-image>
\begin{tikzpicture}[thick,scale=1] 
\draw[step=1cm,color=gray!50] (-3,-4) grid (3,4);
   \draw [black!80,line width=0.5pt,-latex] (0,0) -- (3,0) node [below] at (2.75,0) {$x$};
   \draw [black!80,line width=0.5pt,-latex] (0,0) -- (-3,0);
   \draw [black!80,line width=0.5pt,-latex] (0,0) -- (0,4) node [right] at (0,3.75) {$y$};
   \draw [black!80,line width=0.5pt,-latex] (0,0) -- (0,-4);
\foreach \x/\xtext in { -2/-2, -1/-1, 1/1, 2/2}
    \draw[shift={(\x,0)}] (0pt,3pt) -- (0pt,-3pt); 
\foreach \y/\ytext in {-3/-3, -2/-2, -1/-1, 1/1, 2/2, 3/3}
    \draw[shift={(0,\y)}] (-2pt,0pt) -- (2pt,0pt);
\end{tikzpicture}
      </latex-image>
    </image>
      </sidebyside>
    </figure>
            
  </introduction>  

<task workspace="3cm" xml:id="act-1-3-5-task-1">
        <statement>
      <p>
        Use the definition of the derivative at a point to calculate the value of <m>g'(0)</m>, if it exists.
        Does your answer make sense? Plot the point <m>(0,g'(0))</m> on the graph of <m>g(x)</m> above.
      </p>
    </statement>

  <hint>
    <p>
      Use the definition with <m>a=0</m>.
    </p>
  </hint>
  <answer>
    <p>
      <m>g'(0)=0</m>
    </p>
  </answer>
  <solution>
    <p>
      <md><mrow>g'(0) = \mathstrut \amp \lim_{h \rightarrow 0}\frac{g(0+h)-g(0)}{h} </mrow>
        <mrow> = \mathstrut \amp \lim_{h \rightarrow 0} \frac{g(h)-g(0)}{h} </mrow>
        <mrow> = \mathstrut \amp \lim_{h \rightarrow 0} \frac{|h^2-4|-|0^2-4|}{h} </mrow>
        <mrow> = \mathstrut \amp \lim_{h \rightarrow 0} \frac{-(h^2-4)-4}{h} </mrow>
        <mrow> = \mathstrut \amp \lim_{h \rightarrow 0} \frac{-h^2}{h} </mrow>
        <mrow> = \mathstrut \amp \lim_{h \rightarrow 0} -h </mrow>
        <mrow> = \mathstrut \amp 0</mrow>
      </md>
      This follows since <m>h^2-4 &lt; 0</m> for <m>h</m> near 0.  So <m>(0,g'(0))=(0,0)</m>.  
    </p>
  </solution>
    </task>

<task workspace="3cm" xml:id="act-1-3-5-task-2">
  <statement>
      <p>
        Calculate, if it exists, the value of <m>g'(1)</m>.
        Plot the point <m>(1,g'(1))</m> on the graph of <m>g(x)</m>.
      </p>
    </statement>
    <hint>
      <p>
        Use the definition with <m>a=1</m>.
      </p>
    </hint>
    <answer>
      <p>
        <m>g'(1)=-2</m>
      </p>
    </answer>
    <solution>
      <p>
             <md><mrow>g'(1) = \mathstrut \amp \lim_{h \rightarrow 0}\frac{g(1+h)-g(1)}{h} </mrow>
        <mrow> = \mathstrut \amp \lim_{h \rightarrow 0} \frac{|(1+h)^2-4|-|1^2-4|}{h} </mrow>
        <mrow> = \mathstrut \amp \lim_{h \rightarrow 0} \frac{-((1+h)^2-4)-3}{h} </mrow>
        <mrow> = \mathstrut \amp \lim_{h \rightarrow 0} \frac{-2h-h^2}{h} </mrow>
        <mrow> = \mathstrut \amp \lim_{h \rightarrow 0} -2-h </mrow>
        <mrow> = \mathstrut \amp -2</mrow>
      </md>
      This follows since <m>(1+h)^2-4 &lt; 0</m> for <m>h</m> near 0.  So <m>(1,g'(1))=(1,-2)</m>.
      </p>
    </solution>
  </task>

<task workspace="3cm" xml:id="act-1-3-5-task-3">
  <statement>
    <p>
      Calculate, if it exists, the value of <m>g'(2)</m>.
        Again, illustrate your answer on the graph of <m>g(x)</m>.
    </p>

    <p>
        Note: <m>\displaystyle \lim_{h \rightarrow 0}\frac{g(2+h)-g(2)}{h}</m> is a two-sided limit.
        We investigate the value from each side.
      </p>

            <p>
        <m>\displaystyle \lim_{h \rightarrow 0^-}\frac{g(2+h)-g(2)}{h}=</m>
      </p>

      <p>
        <m>\displaystyle \lim_{h \rightarrow 0^+}\frac{g(2+h)-g(2)}{h}=</m>
      </p>
  </statement>
  <hint>
    <p>
      The absolute value function behaves differently for <m>h</m> positive and <m>h</m> negative.
    </p>
  </hint>
  <answer>
    <p>
      <m>g'(2)</m> does not exist
    </p>
  </answer>
  <solution>
    <p>
        <md><mrow>g'(2) = \mathstrut \amp \lim_{h \rightarrow 0^-}\frac{g(2+h)-g(2)}{h} </mrow>
        <mrow> = \mathstrut \amp \lim_{h \rightarrow 0^-} \frac{|(2+h)^2-4|-|2^2-4|}{h} </mrow>
        <mrow> = \mathstrut \amp \lim_{h \rightarrow 0^-} \frac{-(4+4h+h^2-4)}{h} </mrow>
        <mrow> = \mathstrut \amp \lim_{h \rightarrow 0^-} \frac{-4h-h^2}{h} </mrow>
        <mrow> = \mathstrut \amp \lim_{h \rightarrow 0^-} -4-h </mrow>
        <mrow> = \mathstrut \amp -4</mrow>
      </md>
      since <m>(2+h)^2 &lt; 4</m> for <m>h &lt; 0</m>.  But then we also have the following:
        <md><mrow>g'(2) = \mathstrut \amp \lim_{h \rightarrow 0^+}\frac{g(2+h)-g(2)}{h} </mrow>
        <mrow> = \mathstrut \amp \lim_{h \rightarrow 0^+} \frac{|(2+h)^2-4|-|2^2-4|}{h} </mrow>
        <mrow> = \mathstrut \amp \lim_{h \rightarrow 0^+} \frac{4+4h+h^2-4}{h} </mrow>
        <mrow> = \mathstrut \amp \lim_{h \rightarrow 0^+} \frac{4h+h^2}{h} </mrow>
        <mrow> = \mathstrut \amp \lim_{h \rightarrow 0^+} 4+h </mrow>
        <mrow> = \mathstrut \amp 4</mrow>
      </md>
      since <m>(2+h)^2 &gt; 4</m> if <m>h &gt; 0</m>.  So <m>g'(2)</m> does not exist since the two one-sided limits differ.  
    </p>
  </solution>
</task>

<task workspace="3cm" xml:id="act-1-3-5-task-4">
  <statement>
      <p>
        Using symmetry, make a conjecture about the values of <m>g'(-1)</m> and <m>g'(-2)</m> and plot the corresponding ordered pairs on the graph of <m>g(x)</m>.
      </p>
  </statement>
  <answer>
    <p>
      <m>g'(-1)=2</m> and <m>g'(-2)</m> will not exist.
    </p>
  </answer>
</task>
      



<task workspace="3cm" xml:id="act-1-3-5-task-5">
  <statement>
      <p>
        Using the applet found at <url href="https://www.geogebra.org/m/qwdxbtGF">https://www.geogebra.org/m/qwdxbtGF</url> to check your answers to the above calculations.
        Be sure to also determine if your results make sense graphically.
      </p>
    </statement>
  </task>

</activity>
</worksheet>